theories/Dot/experiments.v
@@ -206,7 +206,7 @@ Section Sec.
     iSpecialize ("Hv" $! (w :: ρ)).
 
     iAssert (□ (⟦ W ⟧ (w :: ρ) w →
-             WP tv v.[to_subst (w :: ρ)] {{ v, ⟦ T ⟧ (w :: ρ) v }}))%I as "#Hv'". {
+             ⟦ T ⟧ₑ (w :: ρ) (tv v.[to_subst (w :: ρ)])))%I as "#Hv'". {
       iIntros "!> #Hw'". iApply "Hv". naive_solver.
     }
 
