theories/saved_interp.v
@@ -11,7 +11,7 @@ From D Require Import tactics.
 Notation savedInterpG Σ A B := (savedAnythingG Σ (A -c> B -c> ▶ ∙)).
 Notation savedInterpΣ A B := (savedAnythingΣ (A -c> B -c> ▶ ∙)).
 Section saved_interp.
-  Context {vls vl: ofeT}.
+  Context {vls vl: Type}.
   Context `{!savedInterpG Σ vls vl}.
   Implicit Type (Φ : vls -c> vl -c> iProp Σ).
 
@@ -56,15 +56,6 @@ Section saved_interp.
     rewrite bi.ofe_fun_equivI; iSpecialize ("Heq" $! v); simpl.
     rewrite bi.later_equivI.
     by iNext; iRewrite -"Heq".
-  Qed.
-
-  Lemma saved_interp_agree_eta γ (Φ Ψ : vls -n> vl -n> iProp Σ) vs v :
-    saved_interp_own γ (λ (vs : vls) (v : vl), Φ vs v) -∗
-    saved_interp_own γ (λ (vs : vls) (v : vl), Ψ vs v) -∗
-    ▷ (Φ vs v ≡ Ψ vs v).
-  Proof.
-    (* Paolo: This manual eta-expansion is needed to get coercions to apply. *)
-    iIntros; by iApply (saved_interp_agree _ (λ a, Φ a) (λ a, Ψ a)).
   Qed.
 End saved_interp.
 
